src/SPNSemantics.v
@@ -86,25 +86,161 @@ Inductive PostSum (spn : Spn) (p : Place) : list Trans -> nat -> Prop :=
       PostSum spn p l sum ->
       PostSum spn p (t :: l) ((post spn t p) + sum).
 
-(** IsSensitized:
+Section IsSensitized.
+
+  (** IsSensitized:
     ∀ t ∈ T, marking m, t ∈ sens(m) if
     ∀ p ∈ P, m(p) ≥ Pre(p, t) ∧ 
              m(p) ≥ Pre_t(p, t) ∧ 
              (m(p) < Pre_i(p, t) ∨ Pre_i(p, t) = 0) *)
 
-Definition IsSensitized
-           (spn : Spn)
-           (marking : list (Place * nat))
-           (t : Trans) : Prop :=
-  IsWellDefinedSpn spn ->
-  MarkingHaveSameStruct spn.(initial_marking) marking ->
-  In t spn.(transs) ->
-  forall (p : Place)
-         (n : nat),
-    In (p, n) marking ->
-    n >= (pre spn t p) /\
-    n >= (test spn t p) /\
-    (n < (inhib spn t p) \/ (inhib spn t p) = 0).
+  Definition IsSensitized
+             (spn : Spn)
+             (marking : list (Place * nat))
+             (t : Trans) : Prop :=
+    IsWellDefinedSpn spn ->
+    MarkingHaveSameStruct spn.(initial_marking) marking ->
+    In t spn.(transs) ->
+    forall (p : Place)
+      (n : nat),
+      In (p, n) marking ->
+      (pre spn t p) <= n  /\
+      (test spn t p) <= n  /\
+      (n < (inhib spn t p) \/ (inhib spn t p) = 0).
+
+  (** Correctness proof for check_pre. *)
+
+  Lemma check_pre_correct :
+    forall (spn : Spn)
+      (marking : list (Place * nat))
+      (p : Place)
+      (t : Trans)
+      (n : nat),
+      IsWellDefinedSpn spn ->
+      MarkingHaveSameStruct spn.(initial_marking) marking ->
+      In (p, n) marking ->
+      check_pre spn marking p t = Some true ->
+      (pre spn t p) <= n.
+  Proof.
+    do 4 intro;
+      functional induction (check_pre spn marking p t) using check_pre_ind;
+      intros.
+    (* General case, all went well. *)
+    - apply get_m_correct in e.
+      (* Proves that ∀ (p, n), (p, nboftokens) ∈ marking ⇒ n = nboftokens. *)
+      unfold IsWellDefinedSpn in H; decompose [and] H; clear H; intros.
+      unfold MarkingHaveSameStruct in H0.
+      unfold NoUnmarkedPlace in H16.
+      unfold NoDupPlaces in H3.
+      rewrite H0 in H16; rewrite H16 in H3.
+      assert (fst (p, n) = fst (p, nboftokens)) by (simpl; reflexivity).
+      generalize (nodup_same_pair marking H3 (p, n) (p, nboftokens) H1 e H); intro.
+      injection H15; intro.
+      rewrite <- H17 in H2; injection H2; intro.
+      apply (leb_complete (pre spn t p) n H18).
+    - inversion H2.
+  Qed.
+
+  (** ∀ spn, marking, pre_places, t, b,
+      map_check_pre_aux spn marking pre_places t b = Some true ⇒
+      b = true.
+   *)
+  Lemma map_check_pre_aux_true_if_true :
+    forall (spn : Spn)
+      (marking : list (Place * nat))
+      (pre_places : list Place)
+      (t : Trans)
+      (b : bool),
+      map_check_pre_aux spn marking pre_places t b = Some true ->
+      b = true.
+  Proof.
+    do 5 intro;
+      functional induction (map_check_pre_aux spn marking pre_places t b)
+                 using map_check_pre_aux_ind;
+      intros.
+    - injection H; auto.
+    - apply IHo in H; apply andb_prop in H; elim H; auto.
+    - inversion H.
+  Qed.
+  
+  (** Correctness proof for map_check_pre_aux. *)
+      
+  Lemma map_check_pre_aux_correct :
+    forall (spn : Spn)
+      (marking : list (Place * nat))
+      (pre_places : list Place)
+      (t : Trans)
+      (b : bool)
+      (neighbours_of_t : Neighbours),
+      IsWellDefinedSpn spn ->
+      MarkingHaveSameStruct spn.(initial_marking) marking ->
+      In (t, neighbours_of_t) spn.(lneighbours) ->
+      incl pre_places (pre_pl neighbours_of_t) ->
+      map_check_pre_aux spn marking pre_places t b = Some true ->
+      forall (p : Place) (n : nat),
+        In p pre_places -> In (p, n) marking -> (pre spn t p) <= n.
+  Proof.
+    do 5 intro;
+      functional induction (map_check_pre_aux spn marking pre_places t b)
+                 using map_check_pre_aux_ind;
+      intros.
+    - inversion H4.
+    - apply in_inv in H4; elim H4; intro.
+      + apply map_check_pre_aux_true_if_true in H3.
+        apply andb_prop in H3; elim H3; intros.
+        rewrite H7 in e0.
+        rewrite H6 in e0.
+        generalize (check_pre_correct spn marking p0 t n H H0 H5 e0); intro.
+        assumption.
+      + apply IHo with (neighbours_of_t := neighbours_of_t);
+          (assumption ||
+           unfold incl in H2;
+           unfold incl; intros;
+           apply in_cons with (a := p) in H7;
+           apply (H2 a H7)).
+    - inversion H3.
+  Qed.
+
+  (** *)
+
+  Lemma map_check_pre_correct :
+    forall (spn : Spn)
+      (marking : list (Place * nat))
+      (pre_places : list Place)
+      (t : Trans)
+      (neighbours_of_t : Neighbours),
+      IsWellDefined spn ->
+      MarkingHaveSameStruct spn.(initial_marking) marking ->
+      In (t, neighbours_of_t) spn.(lneighbours) ->
+      pre_places = (pre_pl neighbours_of_t) ->
+      map_check_pre spn marking pre_places t = Some true ->
+      (forall (p : Place) (n : nat), In (p, n) marking -> (pre spn t p) <= n).
+  Proof.
+    
+  Admitted.
+
+  (** Correctness proof for is_sensitized and IsSensitized *)
+
+  Theorem is_sensitized_correct :
+    forall (spn : Spn)
+      (marking : list (Place * nat))
+      (t : Trans)
+      (neighbours_of_t : Neighbours),
+      MarkingHaveSameStruct spn.(initial_marking) marking ->
+      In (t, neighbours_of_t) spn.(lneighbours) ->
+      is_sensitized spn marking neighbours_of_t t = Some true ->
+      IsSensitized spn marking t.
+  Proof.
+    do 4 intro;
+      functional induction (is_sensitized spn marking neighbours_of_t t)
+                 using is_sensitized_ind;
+      intros.
+    unfold IsSensitized.
+    
+  Qed.
+
+  
+End IsSensitized.
 
 (** SpnIsFirable: 
     ∀ t ∈ T, state s = (m), marking m, t ∈ firable(s) if 
@@ -115,7 +251,7 @@ Definition SpnIsFirable
            (state : SpnState)
            (t : Trans) :=
   IsWellDefinedSpn spn ->
-  MarkingHaveSameStruct spn.(initial_marking) state.(marking) ->
+  IsWellDefinedSpnState spn state ->
   In t spn.(transs) ->
   IsSensitized spn state.(marking) t.
 
@@ -135,10 +271,8 @@ Inductive SpnSemantics (spn : Spn) (s s' : SpnState) : Clock -> Prop :=
 | SpnSemantics_falling_edge :
     
     IsWellDefinedSpn spn ->
-    incl s.(fired) spn.(transs) ->
-    incl s'.(fired) spn.(transs) ->
-    MarkingHaveSameStruct spn.(initial_marking) s.(marking) ->
-    MarkingHaveSameStruct spn.(initial_marking) s'.(marking) ->
+    IsWellDefinedSpnState spn s ->
+    IsWellDefinedSpnState spn s' ->
     (* Marking stays the same between state s and s'. *)
     s.(marking) = s'.(marking) ->
     (* ∀ t ∉ firable(s') ⇒ t ∉ Fired'  
@@ -206,10 +340,8 @@ Inductive SpnSemantics (spn : Spn) (s s' : SpnState) : Clock -> Prop :=
 | SpnSemantics_raising_edge :
     
     IsWellDefinedSpn spn ->
-    incl s.(fired) spn.(transs) ->
-    incl s'.(fired) spn.(transs) ->
-    MarkingHaveSameStruct spn.(initial_marking) s.(marking) ->
-    MarkingHaveSameStruct spn.(initial_marking) s'.(marking) ->
+    IsWellDefinedSpnState spn s ->
+    IsWellDefinedSpnState spn s' ->
     (* Fired stays the same between state s and s'. *)
     s.(fired) = s'.(fired) ->
     (* M' = M - ∑ (pre(t_i) - post(t_i)), ∀ t_i ∈ Fired *)
@@ -221,3 +353,51 @@ Inductive SpnSemantics (spn : Spn) (s s' : SpnState) : Clock -> Prop :=
         In (p, n - preSum + postSum) s'.(marking)) ->
     
     SpnSemantics spn s s' raising_edge.
+
+(** Correctness proof between spn_cycle and SpnSemantics_falling_edge. *)
+
+Theorem spn_semantics_falling_edge_correct :
+  forall (spn : Spn)
+    (s s' s'' : SpnState),
+    IsWellDefinedSpn spn ->
+    IsWellDefinedSpnState spn s ->
+    IsWellDefinedSpnState spn s' ->
+    IsWellDefinedSpnState spn s'' ->
+    spn_cycle spn s = Some (s', s'') ->
+    SpnSemantics spn s s' falling_edge.
+Proof.
+  do 2 intro;
+    functional induction (spn_cycle spn s) using spn_cycle_ind;
+    intros.
+  - apply SpnSemantics_falling_edge.
+    (* Trivial proof, IsWellDefinedSpn. *)
+    + assumption.
+    (* Trivial proof, IsWellDefinedSpnState. *)
+    + assumption.
+    (* Trivial proof, IsWellDefinedSpnState. *)
+    + assumption.
+    (* Proves s.(marking) = s'.(marking) *)
+    + apply spn_map_fire_same_marking in e.
+      injection H3; intros; rewrite <- H5; assumption.
+    (*  *)
+    + unfold spn_map_fire in e; unfold spn_map_fire_aux in e.
+      injection H3; intros; rewrite <- H5.
+  - inversion H3.
+  - inversion H3.
+Qed.
+
+(** Correctness proof between spn_cycle and SpnSemantics_raising_edge. *)
+
+Theorem spn_semantics_raising_edge_correct :
+  forall (spn : Spn)
+         (s s' s'' : SpnState),
+    IsWellDefinedSpn spn ->
+    IsWellDefinedSpnState spn s ->
+    IsWellDefinedSpnState spn s' ->
+    IsWellDefinedSpnState spn s'' ->
+    spn_cycle spn s = Some (s', s'') ->
+    SpnSemantics spn s' s'' raising_edge.
+Proof.
+  do 2 intro.
+  functional induction (spn_cycle spn s) using spn_cycle_ind; intros.
+Qed.
